examples/low-level/sieve.fst
@@ -17,15 +17,6 @@ open ListSet
 val divides : pos -> nat -> Tot bool
 let divides divisor n = ((n % divisor) = 0)
 
-val hasDivisorsSmallerThan : nat -> nat -> Tot bool
-let rec hasDivisorsSmallerThan n bnd =
-match bnd with
-| 0 ->  (assert (9%7=2)); false
-| _ -> (divides bnd n) || (hasDivisorsSmallerThan n (bnd-1))
-
-val isPrime2 : nat -> Tot bool
-let isPrime2 n = hasDivisorsSmallerThan n n
-
 type isPrime n = forall (m:nat). ((2<m /\ m<n) ==> not (divides m n))
 
 (*this program has nested loops. first, we define the inner loop*)
@@ -33,14 +24,16 @@ type isPrime n = forall (m:nat). ((2<m /\ m<n) ==> not (divides m n))
 (*Suppose we are at the m^th iteration in the outer loop*)
 
 (*in a simplified version both inner and outer guards are same; just different variables*)
-type guardLC (n:nat) (li : ref nat) (lo : ref nat)
+type guardLC (n:nat) (lo : ref nat) (li : ref nat)
 (m:smem) =
-  (refExistsInMem li m) && (refExistsInMem lo m) && (((loopkupRef li m) * (loopkupRef lo m) < n))
+  (refExistsInMem li m) && (refExistsInMem lo m) &&
+    (((loopkupRef li m) * (loopkupRef lo m) < n))
 
-val guard :  n:nat -> li:(ref nat) -> lo:(ref nat)  -> unit
+val guard :  n:nat -> lo:(ref nat) -> li:(ref nat)  -> unit
   -> whileGuard (fun m ->  (refExistsInMem li m) /\ (refExistsInMem lo m))
                 (guardLC n li lo)
-let guard n li lo u = (memread li * memread lo < n)
+let guard n li lo u =
+  (memread li * memread lo < n)
 (* the guard of a while loop is not supposed to change the memory*)
 
 type vector (a:Type) (n:nat) = (k:nat{k<n}) -> Tot a
@@ -67,46 +60,27 @@ match bound with
 (*li is the counter for the inner loop; lo is for the outer one*)
 (*the inner loop invariant says that cells lo*0, lo*1, lo*2 ....lo*(li-1) (first li multiples of lo) are marked.*)
 
-#set-options "--initial_fuel 100 --max_fuel 1000 --initial_ifuel 100 --max_ifuel 1000"
-
-type  innerLoopInv (n:nat) (lo: ref nat) (li : ref nat) (res:ref ((k:nat{k<n}) -> Tot bool)) (m:smem) =
-  (guardLC n li lo m)
-  /\ (refExistsInMem res m)
-  /\  ~(li=lo) /\ ~(li==res) /\ ~(lo==res)
-  /\ (forall (k:nat).
-        (k < (loopkupRef li m)) ==> (marked n (loopkupRef res m) ((loopkupRef lo m)*k)))
+(*#set-options "--initial_fuel 100 --max_fuel 100 --initial_ifuel 100 --max_ifuel 100"*)
 
 val mark : n:nat -> ((k:nat{k<n}) -> Tot bool) -> index:nat{index<n} -> Tot ((k:nat{k<n}) -> Tot bool)
 let mark n f index =
   (fun indx -> if (indx= index) then true else f indx)
 
-(*we are inside a loop, so, we have a fresh stack at each iteration of the loop.
- we store li there. creating li is a part of the outer loop*)
+(*using hetrogeneous lists, one can extend this to the general (n-ary) case*)
+type distinctRefsExists3
+  (#a:Type) (#b:Type) (#c:Type) (m:smem)
+  (ra:ref a) (rb: ref b) (rc: ref c)  =
+  (refExistsInMem ra m) /\ (refExistsInMem rb m) /\ (refExistsInMem rc m) /\ (ra=!=rb) /\ (rb=!=rc) /\ (ra=!=rc)
 
-val testAliasing : n:nat -> ((k:nat{k<n}) -> Tot bool) -> SST unit (fun  _  -> True) (fun _ _ _ -> True)
-let testAliasing n initv =
-  pushStackFrame ();
-  let li: ref nat = salloc 1 in
-  let res : ref ((k:nat{k<n}) -> Tot bool) = salloc initv in
-  let resv=memread res in
-    memwrite li 2;
-    let resv2=memread res in
-      assert (resv ==  resv2);
-      popStackFrame ()
+type  innerLoopInv (n:nat) (lo: ref nat) (li : ref nat) (res:ref ((k:nat{k<n}) -> Tot bool)) (m:smem) =
+  (refExistsInMem li m) && (refExistsInMem lo m)
+     && (((loopkupRef li m)-1)*(loopkupRef lo m) < n)
+  /\ (refExistsInMem res m)
+  /\  (li=!=lo) /\ (li=!=res) /\ (lo=!=res)
+  /\ (forall (k:nat).
+        (k < (loopkupRef li m)) ==> (marked n (loopkupRef res m) ((loopkupRef lo m)*k)))
 
-val testAliasing2 : n:nat
- -> li : ref nat
- -> res : ref ((k:nat{k<n}) -> Tot bool)
- -> SST unit
-          (requires (fun  m  -> refExistsInMem res m /\ refExistsInMem li m /\ (li=!=res)))
-          (ensures (fun _ _ _ -> True))
-let testAliasing2 n li res =
-  let resv=memread res in
-    memwrite li 2;
-    let resv2=memread res in
-      assert (resv ==  resv2)
-
-val innerLoop : n:nat
+val innerLoop : n:nat{n>1}
   -> lo: ref nat
   -> li : ref nat
   -> res : ref ((k:nat{k<n}) -> Tot bool)
@@ -115,17 +89,17 @@ val innerLoop : n:nat
                   /\ (forall (k:nat). (k * (loopkupRef lo m1) < n)  ==> marked n (loopkupRef res m1) ((loopkupRef lo m1)*k))
                   )
 
-(*let innerLoop n lo li res =
+let innerLoop n lo li res =
   scopedWhile
     (innerLoopInv n lo li res)
-    (fun m -> (refExistsInMem li m) /\ ((loopkupRef li m) < n))
-    (fun u -> (memread li < n))
+    (guardLC n lo li)
+    (fun u -> (memread li * memread lo < n))
     (fun u ->
       let liv = memread li in
       let lov = memread lo in
       let resv = memread res in
       memwrite li (liv+1);
-      memwrite res (mark n resv (lov * liv)))*)
+      memwrite res (mark n resv (lov * liv)))
 
       (*let resv2=memread res in
       assert (resv2==resv);*)
